Iris/IrisTest/Embedding.lean
@@ -70,59 +70,69 @@ example [BIUpdate PROP1]
   Tests `FromModal` instances with the selector not fixed.
   The default instance `modality_embed` is used.
 -/
-/-- info: solution: FromModal InOut.out True modality_embed
-⎡<affine> P⎤ ⎡<affine> P⎤ iprop(<affine> P), new goals: [] -/
-#guard_msgs in
+/-- info: solution:
+  FromModal FromModal.ModalityStatus.matchGoal True modality_embed
+    ⎡<affine> P⎤ ⎡<affine> P⎤ iprop(<affine> P), new goals: []
+-/
+#guard_msgs (whitespace := lax) in
 variable (P : PROP1) in
-#ipm_synth FromModal .out (α := PROP2) _ _ _ iprop(⎡<affine> P⎤ : PROP2) _
+#ipm_synth FromModal .matchGoal (α := PROP2) _ _ _ iprop(⎡<affine> P⎤ : PROP2) _
 
 /-
   Tests `FromModal` instances with the selector fixed: the low priority
   instances are reachable only once the selector rules out `modality_embed`.
 -/
 /-- info: solution:
-FromModal InOut.out True modality_intuitionistically iprop(□ P) ⎡□ P⎤ ⎡P⎤, new goals: [] -/
-#guard_msgs in
+FromModal FromModal.ModalityStatus.matchGoal True
+  modality_intuitionistically iprop(□ P) ⎡□ P⎤ ⎡P⎤, new goals: []
+-/
+#guard_msgs (whitespace := lax) in
 variable (P : PROP1) in
-#ipm_synth FromModal .out _ _ iprop(□ P) iprop(⎡□ P⎤ : PROP2) _
+#ipm_synth FromModal .matchGoal _ _ iprop(□ P) iprop(⎡□ P⎤ : PROP2) _
 
 /-
   Tests `FromModal` synthesis that is done by `fromModal_intuitionistically_embed`,
   with `io = InOut.in`.
 -/
 /-- info: solution:
-FromModal InOut.in True modality_intuitionistically iprop(□ P) iprop(□ P) P, new goals: [] -/
-#guard_msgs in
+FromModal FromModal.ModalityStatus.known True
+  modality_intuitionistically iprop(□ P) iprop(□ P) P, new goals: []
+-/
+#guard_msgs (whitespace := lax) in
 variable (P : PROP1) in
-#ipm_synth FromModal .in _ modality_intuitionistically iprop(□ P) iprop(□ P : PROP1) _
+#ipm_synth FromModal .known _ modality_intuitionistically iprop(□ P) iprop(□ P : PROP1) _
 
 /- Tests `FromModal` synthesis with `io = InOut.in` along with an unfixed selector. -/
 /-- info: solution:
-FromModal InOut.in True modality_id iprop(|==> P) iprop(|==> P) P, new goals: [] -/
-#guard_msgs in
+FromModal FromModal.ModalityStatus.known True modality_id
+  iprop(|==> P) iprop(|==> P) P, new goals: []
+-/
+#guard_msgs (whitespace := lax) in
 variable (P : PROP1) [BIUpdate PROP1] in
-#ipm_synth FromModal .in (α := PROP1) _ modality_id _ iprop(|==> P : PROP1) _
+#ipm_synth FromModal .known (α := PROP1) _ modality_id _ iprop(|==> P : PROP1) _
 
 /-
   Tests `FromModal` synthesis with nested embeddings.
 -/
 /-- info: solution:
-FromModal InOut.out True modality_affinely iprop(<affine> P) ⎡⎡<affine> P⎤⎤ ⎡⎡P⎤⎤, new goals: [] -/
-#guard_msgs in
+FromModal FromModal.ModalityStatus.matchGoal True modality_affinely
+  iprop(<affine> P) ⎡⎡<affine> P⎤⎤ ⎡⎡P⎤⎤, new goals: []
+-/
+#guard_msgs (whitespace := lax) in
 variable {PROP3 : Type u} [BI PROP3] [BiEmbed PROP2 PROP3] (P : PROP1) in
-#ipm_synth FromModal .out _ _ iprop(<affine> P) iprop(⎡(⎡<affine> P⎤ : PROP2)⎤ : PROP3) _
+#ipm_synth FromModal .matchGoal _ _ iprop(<affine> P) iprop(⎡(⎡<affine> P⎤ : PROP2)⎤ : PROP3) _
 
 /-
   Tests `FromModal` synthesis with the `InOut` parameter not matching the fact
   that `PROP1` is supplied.
 -/
 /-- error:
-parameter #1 PROP1 of FromModal InOut.out ?m.7 ?m.8 iprop(□ P) iprop(□ P) ?m.13
-is an out parameter that is not an mvar
+parameter #1 PROP1 of FromModal FromModal.ModalityStatus.matchGoal ?m.7 ?m.8 iprop(□ P) iprop(□ P)
+  ?m.13 is an out parameter that is not an mvar
 -/
-#guard_msgs in
+#guard_msgs (whitespace := lax) in
 variable (P : PROP1) in
-#ipm_synth FromModal (PROP1 := PROP1) .out _ _ iprop(□ P) iprop(□ P : PROP1) _
+#ipm_synth FromModal (PROP1 := PROP1) .matchGoal _ _ iprop(□ P) iprop(□ P : PROP1) _
 
 /-
   Same test as about, except `io = InOut.in`.
@@ -131,7 +141,7 @@ variable (P : PROP1) in
 /-- info: None -/
 #guard_msgs in
 variable (P : PROP1) in
-#ipm_synth FromModal .in (α := PROP1) _ _ iprop(□ P) iprop(□ P : PROP1) _
+#ipm_synth FromModal .known (α := PROP1) _ _ iprop(□ P) iprop(□ P : PROP1) _
 
 /-
   Tests `imodintro` with the selection for `FromModal` fixed.
